{
 "cells": [
  {
   "cell_type": "markdown",
   "id": "8039250a-1ab8-4f9a-b296-9c9fbe344abf",
   "metadata": {},
   "source": [
    "# Lecture 1: Assignment\n",
    "Made by Charles Montero <br>\n",
    "BSCS - 1\n",
    "<hr>"
   ]
  },
  {
   "cell_type": "markdown",
   "id": "83d945b7-30c8-42f1-962d-86581e690403",
   "metadata": {},
   "source": [
    "$\\textbf{Assignment}$\n",
    "\n",
    "Instructions:\n",
    "- Use latex.\n",
    "- Write your latex in jupyter notebook.\n",
    "- Push your answer to your github account.\n",
    "- Deadline is 2 weeks before finals.\n",
    "- Fail to submit 2 weeks before finals is an automatic 5.0 for this assignment.\n",
    "- Each problem is 25 points.\n",
    "\n",
    "1. Recall the definition of a rational number, denoted as $\\mathbb{Q}$. Prove that the Euler's number $e = \\Sigma_{k=0}^\\infty \\frac{1}{k!} \\notin \\mathbb{Q}$. A factorial is defined as $k! = (k)(k-1)(k-2)(k-3)..., \\forall k \\in \\mathbb{Z}^+$, note that $0! = 1$. Furthermore, a sum notation $\\Sigma_{k=0}^\\infty k = 0+ 1 + 2 + 3 +....+...$\n",
    "\n",
    "$\\textbf{Answer}$\n",
    "\n",
    "Step 1: Assume, for the sake of contradiction, that $e$ is rational. This means that $e$ can be expressed as a fraction $\\frac{p}{q}$ where $p$ and $q$ are integers with no common factors other than 1, and $q \\neq 0$.\n",
    "\n",
    "Step 2: Recall the definition of $e$ as the sum of the infinite series:\n",
    "\n",
    "\n",
    "$ e = \\Sigma_{k=0}^\\infty \\frac{1}{k!}$\n",
    "​\n",
    " \n",
    "Step 3: Consider the partial sums of the series. Let $S_n$ denote the $n$th partial sum:\n",
    "\n",
    "$S_n = \\Sigma_{k=0}^\\infty \\frac{1}{k!}$\n",
    "\n",
    "Step 4: Recognize that $e$ is defined as the limit of these partial sums as $n$ approaches infinity:\n",
    "\n",
    "$e = \\lim_{n \\to \\infty} S_n$\n",
    " \n",
    "Step 5: Since $e$ is rational, $S_n$ must also approach a rational limit as $n$ goes to infinity.\n",
    "\n",
    "Step 6: Notice that each term in the series $\\frac{1}{k!}$ is positive. Therefore, each partial sum $S_n$ is increasing.\n",
    "\n",
    "Step 7: Consider the factorial terms $k!$. For any $k \\geq 1$, we have $k! > k$, which implies $\\frac{1}{k!} < \\frac{1}{k}$.\n",
    "\n",
    "Step 8: Recognize that the series $\\sum_{k=0}^\\infty \\frac{1}{k}$ diverges (known as the harmonic series).\n",
    "\n",
    "Step 9: Since $\\frac{1}{k!} < \\frac{1}{k}$, we can conclude that the series $\\sum_{k=0}^\\infty \\frac{1}{k!}$ converges.\n",
    "\n",
    "Step 10: If $S_n$ converges to a rational number, it must be bounded.\n",
    "\n",
    "Step 11: But the convergence of $\\sum_{k=0}^\\infty \\frac{1}{k!}$ contradicts the unboundedness of the harmonic series.\n",
    "\n",
    "$\\textbf{Conclusion}$: Since assuming $e$ is rational leads to a contradiction, we conclude that $e$ is not rational, i.e., $e \\notin \\mathbb{Q}$.   "
   ]
  },
  {
   "cell_type": "markdown",
   "id": "8e1356d3-5065-4f6f-ab5d-6c6f0a6f73b5",
   "metadata": {},
   "source": [
    "$\\textbf{2. Prove Minkowski's Inequality for sums, $\\forall \\ p>1, (a_k, b_k)>0$:}$\n",
    "\\begin{gather} \n",
    "\\begin{bmatrix} \n",
    "\\Sigma_{k=1}^n |a_k + b_k|^p \n",
    "\\end{bmatrix}^\\frac{1}{p}\n",
    "\\leq\n",
    "\\begin{bmatrix} \n",
    "\\Sigma_{k=1}^n |a_k|^p \n",
    "\\end{bmatrix}^ \\frac{1}{p}\n",
    "+\n",
    "\\begin{bmatrix}\n",
    "\\Sigma_{k=1}^n |b_k|^p\n",
    "\\end{bmatrix}^\\frac{1}{p}\n",
    "\\end{gather}\n",
    "\n",
    "$\\text{Answer:}$\n",
    "\n",
    "Step 1: Laws of Exponents (Power raised to a power):\n",
    "\n",
    "- Let $n = $ any base number, then ${(n^p)}^\\frac{1}{p}=n$\n",
    "- We know that ${(n^p)}^\\frac{1}{p}=n$ for any base number $n$, which implies that the $p$-th root of $n^p$ is $n$. Applying this to the sums of $|a_k|^p$ and $|b_k|^p$, we have:\n",
    "\n",
    "\\begin{gather} \n",
    "\\Sigma_{k=1}^n |a_k + b_k|\n",
    "\\leq\n",
    "\\Sigma_{k=1}^n |a_k|\n",
    "+\n",
    "\\Sigma_{k=1}^n |b_k|\n",
    "\\end{gather}\n",
    "\n",
    "Step 2: Property of Summation (Addition)\n",
    "\n",
    "\\begin{gather} \n",
    "\\Sigma_{k=1}^n |a_k + b_k|\n",
    "\\leq\n",
    "\\Sigma_{k=1}^n |a_k| + |b_k|\n",
    "\\end{gather}\n",
    "\n",
    "Step 3: Prove by Triangle Inequality\n",
    "\n",
    "- Disregarding the Sigma Notation we get:\n",
    "\\begin{gather}\n",
    "|a_k + b_k|\n",
    "\\leq\n",
    "|a_k| + b_k| \n",
    "\\end{gather}\n",
    "\n",
    "- Since, $(a_k, b_k) > 0$, then $(a + b) = a + b$, and $|a| = a_k$, $|b| = b$:\n",
    "- Substitute:\n",
    "\\begin{gather}\n",
    "|a + b| = a + b = |a| + |b|\n",
    "\\end{gather}\n",
    "\n",
    "$\\textbf{Conclusion}$: Thus, the inequality is proven."
   ]
  },
  {
   "cell_type": "markdown",
   "id": "38c0bdac-bbf9-4809-91ce-8fa9fe9c481c",
   "metadata": {},
   "source": [
    "$\\textbf{3. Prove the triangle inequality $|x+y| \\leq |x| + |y|, \\forall (x,y) \\in \\mathbb{R}$}$\n",
    "\n",
    "$\\text{Answer:}$\n",
    "\n",
    "Step 1: Definition of an absolute value\n",
    "\n",
    "- Definition\n",
    "\\begin{gather}\n",
    "{|x| = }\n",
    "\\begin{cases}\n",
    "x,&{x \\geq 0}\\\\ -x,&{x < 0}\n",
    "\\end{cases}\n",
    "\\end{gather}\n",
    "\n",
    "- Thus, we must solve for 4 cases:\n",
    "\n",
    "\\begin{gather}\n",
    "\\text{Case 1: }{x \\geq 0, y \\geq 0} \\\\\n",
    "\\text{Case 2: }{x < 0, y < 0} \\\\\n",
    "\\text{Case 3: }{x \\geq 0, y < 0} \\\\\n",
    "\\text{Case 4: }{x < 0, y \\geq 0} \\\\\n",
    "\\end{gather}\n",
    "\n",
    "Case 1: $x \\geq 0, y \\geq 0$\n",
    "\n",
    "- Let, $|x + y| = x + y$, and $|x| = x, |y| = y$\n",
    "- Substitution:\n",
    "\\begin{gather}\n",
    "|x + y| = x + y = |x| + |y|\n",
    "\\end{gather}\n",
    "\n",
    "Case 2: $x < 0, y < 0$\n",
    "\n",
    "- Let, $|x + y| = -(x + y)$, and $|x| = -x, |y| = -y$\n",
    "- Substitution:\n",
    "\\begin{gather}\n",
    "|x + y| = -(x + y) = -x + (-y) = |x| + |y|\n",
    "\\end{gather}\n",
    "\n",
    "Case 3: $x \\geq 0, y < 0$\n",
    "\n",
    "- Let, $|x| = x, |y| = -y$\n",
    "- Substitution:\n",
    "\\begin{gather}\n",
    "|x + y| \\leq x - y\n",
    "\\end{gather}\n",
    "- Since, $x$  is non-negative and $y$ is negative, $x - y$ could be either positive or negative. So, let's consider both possibilities:\n",
    "\n",
    "For $x + y \\geq 0$:\n",
    "\\begin{gather}\n",
    "x + y \\leq x - y \\\\  \n",
    "y \\leq -y \n",
    "\\end{gather}\n",
    "\n",
    "For $x + y < 0$:\n",
    "\\begin{gather}\n",
    "-(x + y) \\leq x - y \\\\\n",
    "-x - y \\leq x - y \\\\\n",
    "-x \\leq x\n",
    "\\end{gather}}\n",
    "\n",
    "Case 4: $x < 0, y \\geq 0$\n",
    "\n",
    "- Let, $|x| = -x, |y| = y$\n",
    "- Substitution:\n",
    "\\begin{gather}\n",
    "|x + y| \\leq -x + y\n",
    "\\end{gather}\n",
    "- Solve for sub-cases of $|x + y|$:\n",
    "\\begin{gather}\n",
    "x + y, x + y \\geq 0 \\\\\n",
    "-(x + y), x + y < 0 \\\\\n",
    "\\end{gather}\n",
    "\n",
    "For $x + y \\geq 0$:\n",
    "\\begin{gather}\n",
    "x + y \\leq -x + y \\\\\n",
    "x \\leq -x\n",
    "\\end{gather}\n",
    "\n",
    "For $x + y < 0$:\n",
    "\\begin{gather}\n",
    "-(x + y) \\leq -x + y \\\\\n",
    "-x - y \\leq -x + y \\\\\n",
    "-y \\leq y\n",
    "\\end{gather}\n",
    "\n",
    "$\\textbf{Conclusion}$: Therefore, in all cases, $|x+y| \\leq |x| + |y| \\in \\mathbb{R} $"
   ]
  },
  {
   "cell_type": "markdown",
   "id": "d1182961-93b4-4ebc-9a71-2e3119c2c6ff",
   "metadata": {},
   "source": [
    "$\\textbf{4. Prove Sedrakayan's Lemma $\\forall u_i, v_i \\in \\mathbb{R}^+$:}$\n",
    "\n",
    "\\begin{gather}\n",
    "\\frac{(\\Sigma_{i=1}^n u_i)^2}{\\Sigma_{i=1}^n v_i}\n",
    "\\leq\n",
    "\\Sigma_{i=1}^n \\frac{(u_i)^2}{v_i}\n",
    "\\end{gather}\n",
    "\n",
    "$\\text{Answer:}$\n",
    "\n",
    "#### Solution:\n",
    "\n",
    "\n",
    "Step 1: To prove Sedrakayan’s Lemma directly, we need to demonstrate that for all $(u_i, v_i \\in \\mathbb{R}^+)$, the inequality\n",
    "\n",
    "$$\\left(\\frac{\\sum_{i=1}^n u_i}{\\sum_{i=1}^n v_i}\\right)^2 \\leq \\frac{\\sum_{i=1}^n (u_i)^2}{v_i}$$\n",
    "\n",
    "holds true. \n",
    "\n",
    "Step 2: The ***Cauchy-Schwarz Inequality*** states that for any real numbers $(a_i)$ and $(b_i)$, \n",
    "\n",
    "$$\\left(\\sum_{i=1}^n a_i b_i\\right)^2 \\leq \\left(\\sum_{i=1}^n (a_i)^2\\right) \\left(\\sum_{i=1}^n (b_i)^2\\right)$$\n",
    "\n",
    "Step 3: Let $a_i = \\sqrt{u_i}$ and $b_i = \\frac{1}{\\sqrt{v_i}}$. Then, the Cauchy-Schwarz Inequality becomes\n",
    "\n",
    "$$\\left(\\sum_{i=1}^n \\sqrt{u_i} \\cdot \\frac{1}{\\sqrt{v_i}}\\right)^2 \\leq \\left(\\sum_{i=1}^n u_i\\right) \\left(\\sum_{i=1}^n \\frac{1}{v_i}\\right)$$\n",
    "\n",
    "#### Simplify:\n",
    "\n",
    "Step 4: The *left-hand side* simplifies to \n",
    "\n",
    "$$\\left(\\frac{\\sum_{i=1}^n u_i}{\\sum_{i=1}^n v_i}\\right)^2$$\n",
    "\n",
    "Step 5: The *right-hand side* simplifies to \n",
    "\n",
    "$$\\frac{\\sum_{i=1}^n (u_i)^2}{v_i}$$\n",
    "\n",
    "Therefore, since the left-hand side is less than or equal to the right-hand side, we have proven Sedrakayan’s Lemma.\n",
    "\n"
   ]
  },
  {
   "cell_type": "markdown",
   "id": "a4ccdd07-0627-4ede-84ef-d21f0b9e32f4",
   "metadata": {},
   "source": [
    "1. Consider the functions $f(x) = 2x+1$, $g(x)=2y-1$, $j(x) = |f(x)+g(x)|$, and $h(x) = j(x)^2$, show for the following        inequality that:\n",
    "\n",
    "\\begin{gather}\n",
    "\\sqrt{|f(x)|^2} \\geq \\sqrt{h(x)} - \\sqrt{|g(x)|^2}, \\forall (x,y) \\in \\mathbb{Z}^+\n",
    "\\end{gather}\n",
    "\n",
    "2. Prove Sedrakayan's Lemma if $u_i, v_i$ are square roots of an even integers:\n",
    "\\begin{gather}\n",
    "\\frac{(\\Sigma_{i=1}^n u_i)^2}{\\Sigma_{i=1}^n v_i}\n",
    "\\leq\n",
    "\\Sigma_{i=1}^n \\frac{(u_i)^2}{v_i}\n",
    "\\end{gather}"
   ]
  },
  {
   "cell_type": "markdown",
   "id": "b827aba9-881c-45ca-ad7b-11c66c4be365",
   "metadata": {},
   "source": [
    "$\\textbf{1. Consider the functions $f(x) = 2x+1$, $g(x)=2y-1$, $j(x) = |f(x)+g(x)|$, and $h(x) = j(x)^2$, show for the following inequality that:}$\n",
    "\n",
    "\\begin{gather}\n",
    "\\sqrt{|f(x)|^2} \\geq \\sqrt{h(x)} - \\sqrt{|g(x)|^2}, \\forall (x,y) \\in \\mathbb{Z}^+\n",
    "\\end{gather}"
   ]
  },
  {
   "cell_type": "markdown",
   "id": "3c2c2698-fc04-47f6-be58-5cf896a7d38b",
   "metadata": {},
   "source": [
    "$\\textbf{Proof:}$\n",
    "\n",
    "$\\textbf{Step 1: Substitution}$\n",
    "\n",
    "\\begin{equation}\n",
    "\\sqrt{|f(x)|^2} \\geq \\sqrt{|f(x) + g(x)|^2} - \\sqrt{|g(x)|^2}\n",
    "\\end{equation}\n",
    "\n",
    "$\\textbf{Step 2: Minkowski's Inequality for Sums}$\n",
    "\n",
    "\\begin{equation}\n",
    "|f(x)| \\geq |f(x) + g(x)| - |g(x)|\n",
    "\\end{equation}\n",
    "\n",
    "$\\textbf{Step 3: Transpose}$\n",
    "\n",
    "\\begin{equation}\n",
    "|f(x)| + |g(x)| \\geq |f(x) + g(x)|\n",
    "\\end{equation}\n",
    "\n",
    "$\\textbf{Step 4: Rearrange to Triangle Inequality}$\n",
    "\n",
    "\\begin{equation}\n",
    "|f(x) + g(x)| \\leq |f(x)| + |g(x)|\n",
    "\\end{equation}\n",
    "\n",
    "$\\textbf{Step 5: Prove with the case $f(x) > 0$ and $g(x) > 0$, Since $\\forall (x,y) \\in \\mathbb{Z}^+$}$\n",
    "\n",
    "\\begin{equation}\n",
    "Let, \\left|f\\left(x\\right)+g\\left(x\\right)\\right|=f\\left(x\\right)+g\\left(x\\right), and |x|=x, |y|=y\n",
    "\\end{equation}\n",
    "\n",
    "$\\textbf{Step 6: Substitute}$\n",
    "\n",
    "\\begin{gather}\n",
    "\\left|f\\left(x\\right)+g\\left(x\\right)\\right|=f\\left(x\\right)+g\\left(x\\right)=\\left|f\\left(x\\right)\\right|+\\left|g\\left(x\\right)\\right|\n",
    "\\end{gather}"
   ]
  },
  {
   "cell_type": "markdown",
   "id": "15b0f78e-0760-49de-907b-0b852aa29af0",
   "metadata": {},
   "source": [
    "$\\textbf{2. Prove Sedrakayan's Lemma if $u_i, v_i$ are square roots of an even integers:}$\n",
    "\n",
    "\\begin{gather}\n",
    "\\frac{(\\Sigma_{i=1}^n u_i)^2}{\\Sigma_{i=1}^n v_i}\n",
    "\\leq\n",
    "\\Sigma_{i=1}^n \\frac{(u_i)^2}{v_i}\n",
    "\\end{gather}"
   ]
  },
  {
   "cell_type": "markdown",
   "id": "a983dc48-6029-41a8-9f03-8499359ce669",
   "metadata": {},
   "source": [
    "To establish Sedrakayan's Lemma when $u_i$ and $v_i$ are square roots of even integers:\n",
    "\n",
    "Let $u_i = \\sqrt{2a_i}$ and $v_i = \\sqrt{2b_i}$, where $a_i$ and $b_i$ are positive integers. Our goal is to demonstrate:\n",
    "\n",
    "$$\n",
    "\\frac{\\left( \\sum_{i=1}^n \\sqrt{2a_i} \\right)^2}{\\sum_{i=1}^n \\sqrt{2b_i}} \\leq \\sum_{i=1}^n \\frac{(2a_i)}{(2b_i)}\n",
    "$$\n",
    "\n",
    "$\\textbf{Step 1: Expand the terms}$\n",
    "\n",
    "$$\n",
    "\\frac{\\left( \\sum_{i=1}^n \\sqrt{2a_i} \\right)^2}{\\sum_{i=1}^n \\sqrt{2b_i}} = \\frac{\\left( \\sum_{i=1}^n \\sqrt{2a_i} \\right) \\left( \\sum_{i=1}^n \\sqrt{2a_i} \\right)}{\\sum_{i=1}^n \\sqrt{2b_i}}\n",
    "$$\n",
    "\n",
    "and\n",
    "\n",
    "$$\n",
    "\\sum_{i=1}^n \\frac{(2a_i)}{(2b_i)} = \\sum_{i=1}^n \\frac{2a_i}{2b_i}\n",
    "$$\n",
    "\n",
    "$\\textbf{Step 2: Rewrite the inequality}$\n",
    "\n",
    "$$\n",
    "\\frac{\\left( \\sum_{i=1}^n \\sqrt{2a_i} \\right)^2}{\\sum_{i=1}^n \\sqrt{2b_i}} \\leq \\sum_{i=1}^n \\frac{\\sqrt{2a_i}^2}{\\sqrt{2b_i}}\n",
    "$$\n",
    "\n",
    "$\\textbf{Step 3: Apply the identity}$ \n",
    "\n",
    "$$\n",
    "\\left( \\sum_{i=1}^n x_i \\right)^2 = \\sum_{i=1}^n x_i^2 + 2 \\sum_{1 \\leq i < j \\leq n} x_i x_j\n",
    "$$\n",
    "\n",
    "Applying this to the numerator, we get:\n",
    "\n",
    "$$\n",
    "\\frac{\\left( \\sum_{i=1}^n \\sqrt{2a_i} \\right)^2}{\\sum_{i=1}^n \\sqrt{2b_i}} = \\frac{\\sum_{i=1}^n (2a_i) + 2 \\sum_{1 \\leq i < j \\leq n} \\sqrt{2a_i} \\sqrt{2a_j}}{\\sum_{i=1}^n \\sqrt{2b_i}}\n",
    "$$\n",
    "\n",
    "$\\textbf{Step 4: Notice that $2 \\sum_{1 \\leq i < j \\leq n} \\sqrt{2a_i} \\sqrt{2a_j}$ is even.}$\n",
    "\n",
    "$\\textbf{Step 5: Combine the terms} $\n",
    "\n",
    "$$\n",
    "\\frac{\\sum_{i=1}^n (2a_i)}{\\sum_{i=1}^n \\sqrt{2b_i}} + \\frac{2 \\sum_{1 \\leq i < j \\leq n} \\sqrt{2a_i} \\sqrt{2a_j}}{\\sum_{i=1}^n \\sqrt{2b_i}} \\leq \\sum_{i=1}^n \\frac{(2a_i)}{\\sqrt{2b_i}}\n",
    "$$\n",
    "\n",
    "$\\textbf{Step 6: Simplify}$\n",
    "\n",
    "$$\n",
    "\\frac{\\sum_{i=1}^n (2a_i)}{\\sum_{i=1}^n \\sqrt{2b_i}} \\leq \\sum_{i=1}^n \\frac{(2a_i)}{\\sqrt{2b_i}}\n",
    "$$\n",
    "\n",
    "Since both sides are non-negative and the numerator of the left-hand side contains the terms of the denominator of the right-hand side, the inequality holds.\n",
    "\n",
    "$\\textbf{Conclusion:}$ Since both sides are non-negative and the numerator of the left-hand side contains the terms of the denominator of the right-hand side, the inequality holds. Thus, Sedrakayan's Lemma is established for $u_i$ and $v_i$ being square roots of even integers.\n"
   ]
  }
 ],
 "metadata": {
  "kernelspec": {
   "display_name": "Python 3 (ipykernel)",
   "language": "python",
   "name": "python3"
  },
  "language_info": {
   "codemirror_mode": {
    "name": "ipython",
    "version": 3
   },
   "file_extension": ".py",
   "mimetype": "text/x-python",
   "name": "python",
   "nbconvert_exporter": "python",
   "pygments_lexer": "ipython3",
   "version": "3.12.3"
  }
 },
 "nbformat": 4,
 "nbformat_minor": 5
}
